Weidenbach_Book/CDCL_NOT.thy
@@ -314,7 +314,7 @@ lemma reduce_trail_to\<^sub>N\<^sub>O\<^sub>T_state_eq\<^sub>N\<^sub>O\<^sub>T_c
   assumes ST: "S \<sim> T"
   shows "reduce_trail_to\<^sub>N\<^sub>O\<^sub>T F S \<sim> reduce_trail_to\<^sub>N\<^sub>O\<^sub>T F T"
 proof -
-  have "clauses(reduce_trail_to\<^sub>N\<^sub>O\<^sub>T F S) = clauses (reduce_trail_to\<^sub>N\<^sub>O\<^sub>T F T)"
+  have "clauses (reduce_trail_to\<^sub>N\<^sub>O\<^sub>T F S) = clauses (reduce_trail_to\<^sub>N\<^sub>O\<^sub>T F T)"
     using ST by auto
   moreover have "trail (reduce_trail_to\<^sub>N\<^sub>O\<^sub>T F S) = trail (reduce_trail_to\<^sub>N\<^sub>O\<^sub>T F T)"
     using trail_eq_reduce_trail_to\<^sub>N\<^sub>O\<^sub>T_eq[of S T F] ST by auto
